src/SF_lemma.v
@@ -1,6 +1,6 @@
 Require Import Recdef. 
-Require sf_spec.
-Require Import sf_tactic.
+Require SF_spec.
+Require Import SF_tactic.
 Require Import RelDec.
 Require Import List.
 Require Import Sorted.
@@ -15,23 +15,23 @@ Variable candidate : Set.
 Variable reldec_candidate : RelDec (@eq candidate).
 Variable reldec_correct_candidate : RelDec_Correct reldec_candidate.
 
-Ltac solve_rcv := sf_tactic.solve_rcv reldec_correct_candidate.
-Ltac intuition_nosplit := sf_tactic.intuition_nosplit reldec_correct_candidate.
+Ltac solve_rcv := SF_tactic.solve_rcv reldec_correct_candidate.
+Ltac intuition_nosplit := SF_tactic.intuition_nosplit reldec_correct_candidate.
 
 
 Lemma next_ranking_cons_or :
 forall b1 bal e x,
-sf_spec.next_ranking candidate e (b1 :: bal) x ->
-sf_spec.next_ranking candidate e [b1] x \/ 
-sf_spec.next_ranking candidate e bal x.
+SF_spec.next_ranking candidate e (b1 :: bal) x ->
+SF_spec.next_ranking candidate e [b1] x \/ 
+SF_spec.next_ranking candidate e bal x.
 intros. inv H; solve_rcv. left.
-destruct H4; solve_rcv. eapply sf_spec.next_ranking_valid; solve_rcv.
-left. eauto. eapply sf_spec.next_ranking_valid; solve_rcv.
+destruct H4; solve_rcv. eapply SF_spec.next_ranking_valid; solve_rcv.
+left. eauto. eapply SF_spec.next_ranking_valid; solve_rcv.
 Qed.
 
 Lemma next_ranking_in :
 forall e bal x,
-  sf_spec.next_ranking candidate e bal x ->
+  SF_spec.next_ranking candidate e bal x ->
   In x bal.
 Proof.
 induction bal; solve_rcv.
@@ -40,40 +40,40 @@ Qed.
 
 Lemma no_viable_candidates_cons :
 forall a b e,
-sf_spec.no_viable_candidates candidate (e) (a ::  b) <->
-(sf_spec.no_viable_candidates candidate e [a] /\
-sf_spec.no_viable_candidates candidate e b).
+SF_spec.no_viable_candidates candidate (e) (a ::  b) <->
+(SF_spec.no_viable_candidates candidate e [a] /\
+SF_spec.no_viable_candidates candidate e b).
 split.
 intros.
-unfold sf_spec.no_viable_candidates in *.
+unfold SF_spec.no_viable_candidates in *.
 split.
 intros. eapply H; eauto. inv H0; simpl in *; intuition.
 intros. eapply H; eauto. simpl. intuition.
 intros. intuition.
-unfold sf_spec.no_viable_candidates in *. simpl in *.
+unfold SF_spec.no_viable_candidates in *. simpl in *.
 intuition. eapply H0; eauto. 
 eapply H1; eauto.
 Qed.
 
 Lemma first_choices_app : 
 forall c l1 l2 x1 x2  r cnd, 
-sf_spec.first_choices c r cnd l1 x1 ->
-sf_spec.first_choices c r cnd l2 x2 ->
-sf_spec.first_choices c r cnd (l1 ++ l2) (x1 + x2).
+SF_spec.first_choices c r cnd l1 x1 ->
+SF_spec.first_choices c r cnd l2 x2 ->
+SF_spec.first_choices c r cnd (l1 ++ l2) (x1 + x2).
 Proof.
 induction l1; intros.
 - simpl in *. inv H. simpl. auto.
 - simpl in *. 
   inv H.
-  + apply sf_spec.first_choices_selected. auto. fold plus.
+  + apply SF_spec.first_choices_selected. auto. fold plus.
     apply IHl1; auto.
-  + apply sf_spec.first_choices_not_selected; auto.
+  + apply SF_spec.first_choices_not_selected; auto.
 Qed.
 
 Lemma first_choices_app_gt :
 forall c l1 l2 x1 x2 r cnd,
-sf_spec.first_choices c r cnd l1 x1 ->
-sf_spec.first_choices c r cnd (l1 ++ l2) (x2) ->
+SF_spec.first_choices c r cnd l1 x1 ->
+SF_spec.first_choices c r cnd (l1 ++ l2) (x2) ->
 x2 >= x1.
 Proof.
 induction l1; intros.
@@ -86,8 +86,8 @@ Qed.
 Lemma first_choices_perm : 
 forall c l1 l2 x r cnd,
 Permutation l1 l2 ->
-sf_spec.first_choices c r cnd l1 x ->
-sf_spec.first_choices c r cnd l2 x.
+SF_spec.first_choices c r cnd l1 x ->
+SF_spec.first_choices c r cnd l2 x.
 Proof.
 induction l1; intros.
 - apply Permutation_nil in H. subst. auto. 
@@ -106,37 +106,37 @@ induction l1; intros.
       - simpl in *. constructor; auto.
       - simpl in *. inv H. 
         + constructor; auto.
-        + apply sf_spec.first_choices_not_selected; auto.
+        + apply SF_spec.first_choices_not_selected; auto.
     }
   + eapply IHl1 in H; eauto.
     { clear - H H3.
       generalize dependent x1. generalize dependent x.
       induction x0; intros.
-      - simpl in *. apply sf_spec.first_choices_not_selected; auto.
+      - simpl in *. apply SF_spec.first_choices_not_selected; auto.
       - simpl in *. inv H.
         + constructor; auto.
-        + apply sf_spec.first_choices_not_selected; auto.
+        + apply SF_spec.first_choices_not_selected; auto.
     }
 Qed.
 
 Lemma selected_participates : forall election (c : candidate) bal  r,
-sf_spec.selected_candidate _ r bal c ->
+SF_spec.selected_candidate _ r bal c ->
 In bal election ->
-sf_spec.participates _ c election.
+SF_spec.participates _ c election.
 Proof.
 induction election; intros.
 inv H0.
 destruct H0. subst.
-unfold sf_spec.participates.
-unfold sf_spec.selected_candidate in H.
+unfold SF_spec.participates.
+unfold SF_spec.selected_candidate in H.
 destruct H. destruct H0.
 exists bal. split; eauto.
 simpl. auto.
 exists x. intuition.
 apply next_ranking_in in H1. auto.
 eapply IHelection in H0.
-unfold sf_spec.participates in H0.
-unfold sf_spec.participates.
+unfold SF_spec.participates in H0.
+unfold SF_spec.participates.
 simpl in *.
 destruct H0.
 exists x. split; auto. intuition.
@@ -146,45 +146,45 @@ eauto.
 Qed.
 
 Lemma participates_cons : forall e a (c : candidate) ,
-        sf_spec.participates _ c [a] \/ sf_spec.participates _ c e <->
-        sf_spec.participates _ c (a :: e).
+        SF_spec.participates _ c [a] \/ SF_spec.participates _ c e <->
+        SF_spec.participates _ c (a :: e).
 Proof.
 split.
 - intros.
   destruct H.
-  + unfold sf_spec.participates in *.
+  + unfold SF_spec.participates in *.
     destruct H. destruct H. destruct H0. destruct H0.
     exists a. simpl in *. intuition.
     subst. exists x0. auto.
-  + unfold sf_spec.participates in *. 
+  + unfold SF_spec.participates in *. 
     destruct  H. intuition. destruct H1. exists x; intuition.
     exists x0; intuition.
 - intros. destruct H.
   destruct H. destruct H0.
   destruct H.
-  +  unfold sf_spec.participates.
+  +  unfold SF_spec.participates.
      subst. left. exists x. intuition.
      exists x0; auto.
-  +  right. unfold sf_spec.participates.
+  +  right. unfold SF_spec.participates.
      exists x. intuition.
      exists x0; auto.
 Qed.
 
 Lemma total_selected_unique : forall r e v v',
-sf_spec.total_selected candidate r e v ->
-sf_spec.total_selected candidate r e v' ->
+SF_spec.total_selected candidate r e v ->
+SF_spec.total_selected candidate r e v' ->
 v= v'.
 Admitted.
 
 Lemma majority_not_0 :
 forall r e x ,
-sf_spec.majority candidate r e x ->
-exists v, sf_spec.first_choices _ r x e v /\ v <> 0.
+SF_spec.majority candidate r e x ->
+exists v, SF_spec.first_choices _ r x e v /\ v <> 0.
 Proof.
 intros.
-unfold sf_spec.majority in *.
-edestruct (sf_spec.sf_first_choices_total _ r e x).
-edestruct (sf_spec.total_selected_total _ r e).
+unfold SF_spec.majority in *.
+edestruct (SF_spec.sf_first_choices_total _ r e x).
+edestruct (SF_spec.total_selected_total _ r e).
 exists x0. intuition.
 subst.
 eapply H in H0; eauto.
@@ -192,15 +192,15 @@ omega.
 Qed.
 
 Lemma update_eliminated_in_rec : forall rec loser c,
-sf_spec.update_eliminated candidate (in_record rec) loser c <->
+SF_spec.update_eliminated candidate (in_record rec) loser c <->
 in_record ([loser] :: rec) c.
 Proof.
 split; intros.
 { induction rec.
-  - unfold sf_spec.update_eliminated in H.
+  - unfold SF_spec.update_eliminated in H.
     intuition. inv H0. destruct H. inv H.
     subst. unfold in_record. exists [c]. intuition; auto.
-  - unfold sf_spec.update_eliminated in  *. intuition.
+  - unfold SF_spec.update_eliminated in  *. intuition.
     unfold in_record in H0. destruct H0. intuition.
     simpl in H2. destruct H2.
     + subst. unfold in_record. exists x. 
@@ -212,7 +212,7 @@ split; intros.
         intuition.
       * exists x. intuition. }
 { unfold in_record in H. destruct H. intuition. simpl in H0.
-  destruct H0. subst. unfold sf_spec.update_eliminated.
+  destruct H0. subst. unfold SF_spec.update_eliminated.
   right. inv H1; auto. inv H.
   left. unfold in_record. eauto. }
 Qed.
@@ -222,7 +222,7 @@ Axiom prop_ext : forall (P Q : Prop),
 
 
 Lemma update_eliminated_in_rec_eq : forall rec loser c,
-sf_spec.update_eliminated candidate (in_record rec) loser c =
+SF_spec.update_eliminated candidate (in_record rec) loser c =
 in_record ([loser] :: rec) c.
 Proof. intros.
 apply prop_ext. apply update_eliminated_in_rec.
@@ -230,18 +230,18 @@ Qed.
 
 
 Lemma update_eliminated_in_rec_eq_noc : forall rec loser,
-sf_spec.update_eliminated candidate (in_record rec) loser =
+SF_spec.update_eliminated candidate (in_record rec) loser =
 in_record ([loser] :: rec).
 intros. extensionality c. apply update_eliminated_in_rec_eq.
 Qed.
 
 Definition continuing2 b rec:=
-exists r, sf_spec.next_ranking candidate rec b r /\ ~sf_spec.overvote candidate r.
+exists r, SF_spec.next_ranking candidate rec b r /\ ~SF_spec.overvote candidate r.
 
 
 Lemma continuing2_continuing : 
 forall b rec,
-continuing2 b rec <-> sf_spec.continuing_ballot candidate rec b.
+continuing2 b rec <-> SF_spec.continuing_ballot candidate rec b.
 Proof.
 intros.
 split.
@@ -250,7 +250,7 @@ unfold continuing2 in *.
 solve_rcv.
 destruct H1. apply H1. exists x. auto.
 destruct H1. solve_rcv.
-eapply sf_spec.next_ranking_unique in H; eauto. subst.
+eapply SF_spec.next_ranking_unique in H; eauto. subst.
 apply H0; eauto.
 intros.
 unfold continuing2.
@@ -265,8 +265,8 @@ Qed.
 
 Lemma continuing_ballot_cons :
 forall r h t,
-sf_spec.continuing_ballot candidate r (h :: t) ->
-sf_spec.continuing_ballot candidate r [h] \/ ((~sf_spec.overvote candidate h) /\ sf_spec.continuing_ballot candidate r t).
+SF_spec.continuing_ballot candidate r (h :: t) ->
+SF_spec.continuing_ballot candidate r [h] \/ ((~SF_spec.overvote candidate h) /\ SF_spec.continuing_ballot candidate r t).
 Proof.
 intros. repeat rewrite <- continuing2_continuing in *.
 induction t. 
@@ -278,28 +278,28 @@ induction t.
   + destruct H5. 
     *  intuition. 
     * left. exists x.
-      intuition. eapply sf_spec.next_ranking_valid.
+      intuition. eapply SF_spec.next_ranking_valid.
       apply H3. auto.
 Qed.
 
 Lemma continuing_ballot_cons2 :
 forall r a b,
-sf_spec.continuing_ballot candidate r [a] ->
-sf_spec.continuing_ballot candidate r (a :: b).
+SF_spec.continuing_ballot candidate r [a] ->
+SF_spec.continuing_ballot candidate r (a :: b).
 Proof.
 intros. rewrite <- continuing2_continuing in *.
 unfold continuing2 in *. destruct H.
 exists x.
 destruct H. intuition.
 clear H0.
-inv H. inv H5. eapply sf_spec.next_ranking_valid; eauto.
+inv H. inv H5. eapply SF_spec.next_ranking_valid; eauto.
 Qed.
 
 Lemma continuing_ballot_cons3 :
 forall t h r
-(OV : ~sf_spec.overvote candidate h), 
-sf_spec.continuing_ballot candidate r t ->
-sf_spec.continuing_ballot candidate r (h :: t).
+(OV : ~SF_spec.overvote candidate h), 
+SF_spec.continuing_ballot candidate r t ->
+SF_spec.continuing_ballot candidate r (h :: t).
 Proof.
 intros. rewrite <- continuing2_continuing in *.
 unfold continuing2 in *.
@@ -309,7 +309,7 @@ exists x. intuition.
 constructor; eauto.
 destruct h. exfalso. solve_rcv. apply H1. solve_rcv.
 exists (c::h). intuition.
-eapply sf_spec.next_ranking_valid. simpl. eauto. 
+eapply SF_spec.next_ranking_valid. simpl. eauto. 
 right. solve_rcv. apply H1. intros. destruct H3. subst. auto.
 destruct (rel_dec_p c x0).
 subst. auto.
@@ -319,13 +319,13 @@ Qed.
 
 Lemma continuing_ballot_rec_cons : 
 forall l r b,
-  sf_spec.continuing_ballot candidate (in_record ([l] :: r)) (b) ->
-   sf_spec.continuing_ballot candidate (in_record r) (b).
+  SF_spec.continuing_ballot candidate (in_record ([l] :: r)) (b) ->
+   SF_spec.continuing_ballot candidate (in_record r) (b).
 Proof.
   intros. induction b.
-  - unfold sf_spec.continuing_ballot in *.  
+  - unfold SF_spec.continuing_ballot in *.  
     intro. apply H. clear H.
-    unfold sf_spec.exhausted_ballot. left. intro.
+    unfold SF_spec.exhausted_ballot. left. intro.
     inv H. inv H1.
   - apply continuing_ballot_cons in H.  
     destruct H.
@@ -337,7 +337,7 @@ Proof.
     destruct H. intuition.
     inv H. constructor; solve_rcv.
     destruct H5. intuition.
-    eapply sf_spec.next_ranking_valid; eauto.
+    eapply SF_spec.next_ranking_valid; eauto.
     right. intro. apply H; clear H.
     unfold in_record in *. solve_rcv.
     intuition.
@@ -346,18 +346,18 @@ Qed.
 
 Lemma next_ranking_cons_or2 :
 forall b1 bal e x,
-sf_spec.next_ranking candidate e (b1 :: bal) x ->
-sf_spec.next_ranking candidate e [b1] x \/ 
-(Forall e b1 /\ sf_spec.next_ranking candidate e bal x).
+SF_spec.next_ranking candidate e (b1 :: bal) x ->
+SF_spec.next_ranking candidate e [b1] x \/ 
+(Forall e b1 /\ SF_spec.next_ranking candidate e bal x).
 intros. inv H; solve_rcv. left.
-destruct H4; solve_rcv. eapply sf_spec.next_ranking_valid; solve_rcv.
-left. eauto. eapply sf_spec.next_ranking_valid; solve_rcv.
+destruct H4; solve_rcv. eapply SF_spec.next_ranking_valid; solve_rcv.
+left. eauto. eapply SF_spec.next_ranking_valid; solve_rcv.
 Qed.
 
 Lemma continuing_ballot_cons4 : (*should be main lemma, don't want to rework proofs :( *)
 forall r h t,
-sf_spec.continuing_ballot candidate r (h :: t) ->
-sf_spec.continuing_ballot candidate r [h] \/ ((~sf_spec.overvote candidate h) /\ sf_spec.continuing_ballot candidate r t /\ Forall r h).
+SF_spec.continuing_ballot candidate r (h :: t) ->
+SF_spec.continuing_ballot candidate r [h] \/ ((~SF_spec.overvote candidate h) /\ SF_spec.continuing_ballot candidate r t /\ Forall r h).
 Proof.
 intros. repeat rewrite <- continuing2_continuing in *.
 induction t. 
@@ -369,37 +369,37 @@ induction t.
   + destruct H5. 
     *  intuition. 
     * left. exists x.
-      intuition. eapply sf_spec.next_ranking_valid.
+      intuition. eapply SF_spec.next_ranking_valid.
       apply H3. auto.
 Qed.
 
 Lemma selected_cons :
 forall r a b c,
-sf_spec.selected_candidate candidate  r (a :: b) c ->
-sf_spec.selected_candidate candidate r [a] c \/
-(Forall r a /\ ~sf_spec.overvote candidate a /\sf_spec.selected_candidate candidate r b c).
+SF_spec.selected_candidate candidate  r (a :: b) c ->
+SF_spec.selected_candidate candidate r [a] c \/
+(Forall r a /\ ~SF_spec.overvote candidate a /\SF_spec.selected_candidate candidate r b c).
 Proof.
 intros.
-unfold sf_spec.selected_candidate in H.
+unfold SF_spec.selected_candidate in H.
 intuition_nosplit. apply continuing_ballot_cons4 in H.
 apply next_ranking_cons_or2 in H0.
 destruct H, H0.
-left. unfold sf_spec.selected_candidate. intuition.
+left. unfold SF_spec.selected_candidate. intuition.
 eauto.
 rewrite <- continuing2_continuing in H.
 unfold continuing2 in H. destruct H. destruct H.
 inv H. inv H8. rewrite Forall_forall in H0. firstorder.
 destruct H. destruct H2. inv H0. inv H9. rewrite Forall_forall in *.
 firstorder.
-right. unfold sf_spec.selected_candidate. intuition.
+right. unfold SF_spec.selected_candidate. intuition.
 eauto.
 Qed.
 
 Lemma first_choices_0_cons :
 forall r c h t,
-sf_spec.first_choices candidate r c (h :: t) 0 <->
-sf_spec.first_choices candidate r c [h] 0 /\
-sf_spec.first_choices candidate r c t 0.
+SF_spec.first_choices candidate r c (h :: t) 0 <->
+SF_spec.first_choices candidate r c [h] 0 /\
+SF_spec.first_choices candidate r c t 0.
 Proof.
 split.
 - intros.
@@ -416,9 +416,9 @@ Lemma next_ranking_record_same :
 forall b x c l r,
   In c x ->
   c <> l ->
-  sf_spec.next_ranking candidate (in_record r) b x ->
-  ~ sf_spec.overvote candidate x ->
-  sf_spec.next_ranking candidate (in_record ([l] :: r)) b x.
+  SF_spec.next_ranking candidate (in_record r) b x ->
+  ~ SF_spec.overvote candidate x ->
+  SF_spec.next_ranking candidate (in_record ([l] :: r)) b x.
 Proof.
 induction b; intros.
 inv H1.
@@ -427,7 +427,7 @@ inv H1.
   auto.
   eapply IHb; eauto.
 - intuition.
-  eapply sf_spec.next_ranking_valid.
+  eapply SF_spec.next_ranking_valid.
   apply H5. right. intro.
   apply H1. solve_rcv. simpl in H3. destruct H3; solve_rcv.
   assert (c0 = l). inv H4. subst; intuition. inv H3. subst. clear H4.
@@ -436,52 +436,52 @@ Qed.
 
 Lemma ne_still_continuing :
 forall b c l  x r,
-sf_spec.next_ranking candidate (in_record r) b x ->
-sf_spec.continuing_ballot candidate (in_record r) b ->
+SF_spec.next_ranking candidate (in_record r) b x ->
+SF_spec.continuing_ballot candidate (in_record r) b ->
 In c x ->
 c <> l ->
-sf_spec.continuing_ballot candidate (in_record ([l] :: r)) b.
+SF_spec.continuing_ballot candidate (in_record ([l] :: r)) b.
 Proof.
 intros. repeat rewrite <- continuing2_continuing in *.
 unfold continuing2 in *. intuition_nosplit.
 exists x0. split; eauto. 
-eapply sf_spec.next_ranking_unique in H; eauto. subst.
+eapply SF_spec.next_ranking_unique in H; eauto. subst.
 eapply next_ranking_record_same; eauto.
 Qed.
 
 Lemma selected_rec_cons :
 forall r b c l,
 c <> l ->
-sf_spec.selected_candidate candidate (in_record r) b c ->
-sf_spec.selected_candidate candidate (in_record ([l]::r)) b c.
+SF_spec.selected_candidate candidate (in_record r) b c ->
+SF_spec.selected_candidate candidate (in_record ([l]::r)) b c.
 intros.
 induction b. solve_rcv.
 apply selected_cons in H0. 
 destruct H0. 
 - clear IHb. 
-  unfold sf_spec.selected_candidate in *.
+  unfold SF_spec.selected_candidate in *.
   intuition_nosplit.
   split. 
   + apply continuing_ballot_cons2. 
   eapply ne_still_continuing; eauto.
   + inv H1. inv H8.
     destruct H7. exists x. intuition.
-    eapply sf_spec.next_ranking_valid; eauto.
-    exists x. intuition. eapply sf_spec.next_ranking_valid; eauto.
+    eapply SF_spec.next_ranking_valid; eauto.
+    exists x. intuition. eapply SF_spec.next_ranking_valid; eauto.
     right. intro. apply H1. rewrite <- continuing2_continuing in *. 
     unfold continuing2 in *. unfold in_record in *. intuition_nosplit. 
     simpl in *. destruct H3; subst; try solve [solve_rcv].
     inv H4; intuition_nosplit. inv H0. inv H10. intuition.
     exfalso. apply H6. solve_rcv.
 - intuition. clear H3. 
-  unfold sf_spec.selected_candidate in *.
+  unfold SF_spec.selected_candidate in *.
   intuition_nosplit. split. 
   rewrite <- continuing2_continuing. unfold continuing2. exists x.
   intuition. constructor; auto. rewrite Forall_forall in *.
   intro. specialize (H1 x0). intro. intuition. 
   solve_rcv.  rewrite <-  continuing2_continuing in *.
   unfold continuing2 in *. intuition_nosplit.
-  eapply sf_spec.next_ranking_unique in H2; eauto. subst.
+  eapply SF_spec.next_ranking_unique in H2; eauto. subst.
   auto.
   exists x. intuition.
   constructor; auto.
@@ -491,9 +491,9 @@ Qed.
 
 Lemma first_choices_rec_0 :
 forall c l r e,
-  sf_spec.first_choices candidate (in_record ([l] :: r)) c e 0 ->
+  SF_spec.first_choices candidate (in_record ([l] :: r)) c e 0 ->
   c <> l ->
-  sf_spec.first_choices candidate (in_record r) c e 0.
+  SF_spec.first_choices candidate (in_record r) c e 0.
 Proof.
 intros.
 induction e.
@@ -510,17 +510,17 @@ Qed.
 Lemma first_choices_0_loser :
 forall c election l,
 ~in_record l c ->
-sf_spec.participates _ c election ->
-sf_spec.first_choices candidate (in_record l) c election 0 ->
-sf_spec.is_loser _ (in_record l) election c.
+SF_spec.participates _ c election ->
+SF_spec.first_choices candidate (in_record l) c election 0 ->
+SF_spec.is_loser _ (in_record l) election c.
 Proof.
-intros. unfold sf_spec.is_loser in *.
+intros. unfold SF_spec.is_loser in *.
 split.
-- unfold sf_spec.viable_candidate. 
+- unfold SF_spec.viable_candidate. 
   split.
   + unfold in_record. intuition_nosplit. apply H. unfold in_record. eauto.
   + auto.
-- intros. eapply sf_spec.sf_first_choices_unique in H1; eauto. subst. omega.
+- intros. eapply SF_spec.sf_first_choices_unique in H1; eauto. subst. omega.
 Qed.
 
 Lemma in_record_nil_nil (c: candidate) :
@@ -698,15 +698,15 @@ Qed.
 Lemma selected_cons' : 
 forall r a b c,
 Forall r a ->
-~sf_spec.overvote _ a ->
-sf_spec.selected_candidate candidate r b c ->
-sf_spec.selected_candidate _ r (a :: b) c.
+~SF_spec.overvote _ a ->
+SF_spec.selected_candidate candidate r b c ->
+SF_spec.selected_candidate _ r (a :: b) c.
 Proof.
 intros. rewrite Forall_forall in *.
 induction b.
 inv H1. intuition_nosplit. 
 destruct H1.  intuition_nosplit.
-unfold sf_spec.selected_candidate.
+unfold SF_spec.selected_candidate.
 split. 
 - rewrite <- continuing2_continuing in *.
   unfold continuing2 in *.
@@ -719,10 +719,10 @@ Qed.
 
 Lemma first_choices_0_not_next :
 forall election c b l rnk
-(OV: ~sf_spec.overvote _ rnk),
- sf_spec.first_choices candidate (in_record l) c election 0 ->
+(OV: ~SF_spec.overvote _ rnk),
+ SF_spec.first_choices candidate (in_record l) c election 0 ->
 In b election ->
-sf_spec.next_ranking candidate (in_record l) b rnk ->
+SF_spec.next_ranking candidate (in_record l) b rnk ->
 ~In c rnk.
 Proof.
 intros.
@@ -739,36 +739,36 @@ destruct H0.
       auto.
     * destruct H6. intuition. inv H. apply H5. clear H5.
       split. rewrite <- continuing2_continuing. unfold continuing2.
-      exists rnk. intuition. eapply sf_spec.next_ranking_valid.
+      exists rnk. intuition. eapply SF_spec.next_ranking_valid.
       apply H4. intuition.
-      exists rnk. intuition. eapply sf_spec.next_ranking_valid. apply H4. intuition.
+      exists rnk. intuition. eapply SF_spec.next_ranking_valid. apply H4. intuition.
 - apply IHelection; auto. inv H. auto.
 Qed.
 
 Lemma not_selected_eliminated :
 forall r c a b,
-~sf_spec.overvote candidate (c :: a) ->
-~sf_spec.selected_candidate _ r ((c :: a)::b) c ->
+~SF_spec.overvote candidate (c :: a) ->
+~SF_spec.selected_candidate _ r ((c :: a)::b) c ->
 r c.
 Proof.
 intros.
-- unfold sf_spec.selected_candidate in H0. rewrite <- continuing2_continuing in H0.
+- unfold SF_spec.selected_candidate in H0. rewrite <- continuing2_continuing in H0.
   destruct (classic (r c)). auto. exfalso.
   apply H0. clear H0. split.
   unfold continuing2. exists (c :: a).
-  intuition. eapply sf_spec.next_ranking_valid with (c := c). 
+  intuition. eapply SF_spec.next_ranking_valid with (c := c). 
   simpl. auto. auto.
   exists (c::a). intuition.
-  apply sf_spec.next_ranking_valid with (c := c). simpl. auto.
+  apply SF_spec.next_ranking_valid with (c := c). simpl. auto.
   intuition.
 Qed.
 
 Lemma rem_0_still_next :
 forall c l  x b election,
-sf_spec.first_choices candidate (in_record [l]) c (election) 0 ->
+SF_spec.first_choices candidate (in_record [l]) c (election) 0 ->
 In b election ->
-sf_spec.next_ranking candidate (in_record [c :: l]) b x ->
-sf_spec.next_ranking candidate (in_record [l]) b x.
+SF_spec.next_ranking candidate (in_record [c :: l]) b x ->
+SF_spec.next_ranking candidate (in_record [l]) b x.
 intros. induction election.
 - inv H0.
 - simpl in H0. destruct H0. 
@@ -787,16 +787,16 @@ intros. induction election.
             * subst. constructor; auto. apply not_selected_eliminated in H3; auto.
               rewrite Forall_forall. intros.
               simpl in H. destruct H. solve_rcv.
-              apply sf_spec.not_overvote_all_same with (c := c0) in H4; simpl; auto.
+              apply SF_spec.not_overvote_all_same with (c := c0) in H4; simpl; auto.
               rewrite Forall_forall in H4. specialize (H4 x0).
               simpl in H4. intuition. subst. auto. apply (fun _ => False).
               apply H0. clear H0. constructor; auto.
               intro. apply H3. apply selected_cons'; auto. apply not_selected_eliminated in H3; auto.
               rewrite Forall_forall. intros. simpl in *. intuition; try solve[solve_rcv].
-              apply sf_spec.not_overvote_all_same with (c := c0) in H4; simpl; auto.
+              apply SF_spec.not_overvote_all_same with (c := c0) in H4; simpl; auto.
               rewrite Forall_forall in H4. specialize (H4 x0). simpl in *. intuition.
               subst. auto. apply (fun _ => False).
-            * constructor; auto. apply sf_spec.not_overvote_all_same with (c := c0) in H4;
+            * constructor; auto. apply SF_spec.not_overvote_all_same with (c := c0) in H4;
                                  simpl; auto.
               rewrite Forall_forall in *.
               intros. simpl in H1. intuition; subst; auto. unfold in_record. exists l.
@@ -805,12 +805,12 @@ intros. induction election.
               apply H0. clear H0. constructor; auto.
               intro. apply H3. apply selected_cons'; auto. 
               rewrite Forall_forall. intros. simpl in *. intuition; try solve[solve_rcv].
-              apply sf_spec.not_overvote_all_same with (c := c0) in H4; simpl; auto.
+              apply SF_spec.not_overvote_all_same with (c := c0) in H4; simpl; auto.
               rewrite Forall_forall in H4. specialize (H4 x0). simpl in *. intuition.
               subst. exists l. simpl. auto. apply (fun _ => False).
         - destruct H6.
-           + eapply sf_spec.next_ranking_valid; eauto.
-           + eapply sf_spec.next_ranking_valid; eauto.
+           + eapply SF_spec.next_ranking_valid; eauto.
+           + eapply SF_spec.next_ranking_valid; eauto.
              right. intro. apply H. unfold in_record in H0. intuition_nosplit.
              exists (c::l). intuition. simpl. inv H0. auto. inv H4.
       }
@@ -819,10 +819,10 @@ Qed.
 
 Lemma rem_0_still_continuing :
 forall election c l b,
-sf_spec.first_choices candidate (in_record [l]) c (election) 0 ->
+SF_spec.first_choices candidate (in_record [l]) c (election) 0 ->
 In b election ->
-sf_spec.continuing_ballot candidate (in_record [c :: l]) b ->
-sf_spec.continuing_ballot candidate (in_record [l]) b.
+SF_spec.continuing_ballot candidate (in_record [c :: l]) b ->
+SF_spec.continuing_ballot candidate (in_record [l]) b.
 intros. rewrite <- continuing2_continuing in *. unfold continuing2 in *.
 intuition_nosplit. exists x. intuition.
 eapply rem_0_still_next; eauto.    
@@ -830,17 +830,17 @@ Qed.
 
 Lemma next_ranking_add_c : 
 forall c l a x election,
-sf_spec.first_choices candidate (in_record [l]) c election 0 ->
+SF_spec.first_choices candidate (in_record [l]) c election 0 ->
 In a election ->
-sf_spec.next_ranking candidate (in_record [l]) a x ->
-sf_spec.next_ranking candidate (in_record [c::l]) a x.
+SF_spec.next_ranking candidate (in_record [l]) a x ->
+SF_spec.next_ranking candidate (in_record [c::l]) a x.
 Admitted.
 
 Lemma total_selected_remove_0 :
 forall election c l t,
-  sf_spec.first_choices candidate (in_record [l]) c election 0 ->
-  sf_spec.total_selected candidate (in_record [c :: l]) election t ->
-  sf_spec.total_selected candidate (in_record [l]) election t.
+  SF_spec.first_choices candidate (in_record [l]) c election 0 ->
+  SF_spec.total_selected candidate (in_record [c :: l]) election t ->
+  SF_spec.total_selected candidate (in_record [l]) election t.
 Proof.
 induction election; intros.
 inv H0. constructor.
@@ -848,7 +848,7 @@ inv H0.
 constructor.
 eapply rem_0_still_continuing; simpl; eauto. simpl. eauto. 
 eapply IHelection; eauto. inv H; auto. constructor; auto.
-unfold sf_spec.exhausted_ballot in *. 
+unfold SF_spec.exhausted_ballot in *. 
 destruct H3.
 left. intro. apply H0. clear H0.
 intuition_nosplit. exists x. eapply next_ranking_add_c; eauto.
@@ -861,39 +861,39 @@ Qed.
 
 Lemma first_choices_remove_0 :
   forall l c x election winner_votes,
-  sf_spec.first_choices candidate (in_record [l]) c election 0 ->
-  sf_spec.first_choices candidate (in_record [c :: l]) x election
+  SF_spec.first_choices candidate (in_record [l]) c election 0 ->
+  SF_spec.first_choices candidate (in_record [c :: l]) x election
                         winner_votes ->
-  sf_spec.first_choices candidate (in_record [l]) x election winner_votes.
+  SF_spec.first_choices candidate (in_record [l]) x election winner_votes.
 Admitted.
 
 Lemma no_majority_remove_0 :
 forall  l election c,
-sf_spec.first_choices candidate (in_record [l]) c election 0 ->
-sf_spec.no_majority candidate (in_record [c :: l]) election ->
-sf_spec.no_majority candidate (in_record [l]) election.
+SF_spec.first_choices candidate (in_record [l]) c election 0 ->
+SF_spec.no_majority candidate (in_record [c :: l]) election ->
+SF_spec.no_majority candidate (in_record [l]) election.
 Proof.
-intros. unfold sf_spec.no_majority in *.
+intros. unfold SF_spec.no_majority in *.
 intro. apply H0. clear H0. 
 destruct H1.
-exists x. unfold sf_spec.majority in *. intros.
+exists x. unfold SF_spec.majority in *. intros.
 apply total_selected_remove_0 in H1; auto.
 apply H0; auto. generalize dependent H2. revert H.  apply first_choices_remove_0.
 Qed.
 
 Lemma not_isloser_nil :
 forall loser r,
-~ sf_spec.is_loser candidate r [] loser. 
+~ SF_spec.is_loser candidate r [] loser. 
 intros. intro.
-unfold sf_spec.is_loser in *.
+unfold SF_spec.is_loser in *.
 intuition. inv H0. inv H2. intuition.
 Qed.
 
 Lemma not_winner_nil :
 forall r winner,
-~sf_spec.winner candidate [] r winner.
+~SF_spec.winner candidate [] r winner.
 intros. intro. inv H. 
-- unfold sf_spec.majority in *.
+- unfold SF_spec.majority in *.
   specialize (H0 0 0). assert (0 * 2 > 0).
   apply H0. constructor. constructor. omega.
 - apply not_isloser_nil in H1. auto.
@@ -906,49 +906,49 @@ Qed.
 
 Lemma not_participates_rec :
   forall c election l winner,
-    ~ sf_spec.participates candidate c (election) ->
-    sf_spec.winner candidate (election) (in_record [c :: l]) winner ->
-    sf_spec.winner candidate (election) (in_record [l]) winner.
+    ~ SF_spec.participates candidate c (election) ->
+    SF_spec.winner candidate (election) (in_record [c :: l]) winner ->
+    SF_spec.winner candidate (election) (in_record [l]) winner.
  Admitted.
 
 Lemma majority_unique :
 forall r e x x',
-sf_spec.majority candidate r e x ->
-sf_spec.majority candidate r e x' ->
+SF_spec.majority candidate r e x ->
+SF_spec.majority candidate r e x' ->
 x = x'.
 Admitted.
 
 Lemma majority_remove_0 :
   forall l c election winner,
-  sf_spec.first_choices candidate (in_record [l]) c (election) 0 ->
-   sf_spec.majority candidate (in_record [c :: l]) (election) winner ->
-   sf_spec.majority candidate (in_record [l]) (election) winner.
+  SF_spec.first_choices candidate (in_record [l]) c (election) 0 ->
+   SF_spec.majority candidate (in_record [c :: l]) (election) winner ->
+   SF_spec.majority candidate (in_record [l]) (election) winner.
 Admitted.
 
 
 Lemma winner_eliminate_0s' :
 forall election  c winner l
 (NODUP : NoDup (c::l)),
-sf_spec.first_choices _ (in_record [l]) c election 0 ->
-sf_spec.winner candidate election (in_record ([c ::l]) ) winner ->
-sf_spec.winner candidate election (in_record [l]) winner.
+SF_spec.first_choices _ (in_record [l]) c election 0 ->
+SF_spec.winner candidate election (in_record ([c ::l]) ) winner ->
+SF_spec.winner candidate election (in_record [l]) winner.
 Proof.
 intros.
 induction election.
 - clear H. inv H0. 
-  + unfold sf_spec.majority in *. specialize (H 0 0). 
+  + unfold SF_spec.majority in *. specialize (H 0 0). 
     assert (0*2 > 0). apply H. constructor; auto. constructor. omega. 
   + apply not_winner_nil in H2. inv H2. 
-- destruct (classic (sf_spec.no_majority candidate (in_record [c :: l]) (a :: election))).
-  + destruct (classic ( sf_spec.participates candidate c (a :: election))). 
-    * apply sf_spec.winner_elimination with (loser := c); auto. 
+- destruct (classic (SF_spec.no_majority candidate (in_record [c :: l]) (a :: election))).
+  + destruct (classic ( SF_spec.participates candidate c (a :: election))). 
+    * apply SF_spec.winner_elimination with (loser := c); auto. 
       apply no_majority_remove_0 in H1; auto.
       apply first_choices_0_loser. inv NODUP. intro. apply H5.
       solve_rcv. inv H3. auto. inv H7. 
       auto. auto. rewrite update_eliminated_in_rec_eq_noc. rewrite in_record_flatten_eq.
       simpl. rewrite app_nil_r. auto. 
     * eapply not_participates_rec; eauto.
-  + unfold sf_spec.no_majority in *.  apply NNPP in H1. destruct H1.
+  + unfold SF_spec.no_majority in *.  apply NNPP in H1. destruct H1.
     inv H0. assert (x = winner). eapply majority_unique; eauto. subst.
     constructor.  apply majority_remove_0 in H2. auto.
     auto.
@@ -958,24 +958,24 @@ Qed.
 
 Lemma first_choices_0_rev:
 forall l a election,
-(forall c, In c l -> sf_spec.first_choices candidate (in_record []) c election 0) ->
-sf_spec.first_choices candidate (in_record []) a election 0 ->
-sf_spec.first_choices candidate (in_record [l]) a election 0.
+(forall c, In c l -> SF_spec.first_choices candidate (in_record []) c election 0) ->
+SF_spec.first_choices candidate (in_record []) a election 0 ->
+SF_spec.first_choices candidate (in_record [l]) a election 0.
 Admitted.
 
 Lemma winner_eliminate_0s :
 forall election winner l
 (NODUP : NoDup l),
-(forall c, in_record [l] c -> sf_spec.first_choices _ (in_record []) c election 0) ->
-sf_spec.winner candidate election (in_record [l] ) winner ->
-sf_spec.winner candidate election (in_record []) winner.
+(forall c, in_record [l] c -> SF_spec.first_choices _ (in_record []) c election 0) ->
+SF_spec.winner candidate election (in_record [l] ) winner ->
+SF_spec.winner candidate election (in_record []) winner.
 Proof.
   induction l; intros. rewrite in_record_nil_nil_eq. auto.
   apply winner_eliminate_0s' in H0; auto. 
   apply IHl; auto. inv NODUP; auto. intros.
   specialize (H c). apply H. destruct H1. intuition.
   exists (a::l). simpl; intuition. inv H2; auto. inv H1.
-  assert (sf_spec.first_choices candidate (in_record []) a election 0). 
+  assert (SF_spec.first_choices candidate (in_record []) a election 0). 
   apply H. exists (a::l); simpl; intuition.
   apply first_choices_0_rev; auto. intros. apply H.
   exists (a :: l). simpl; auto.
