src/SF_tests.v
@@ -1,4 +1,4 @@
-Require Import sf_imp.
+Require Import SF_imp.
 Require Import RelDec.
 Require Import List.
 Import ListNotations.
